src/RqRsRed.v
@@ -18,19 +18,9 @@ Section InsideTree.
 
   Hypothesis (Hrrs: RqRsSys dtr sys).
 
-  Ltac exfalso_midx :=
-    match goal with
-    | [H1: rqEdgeUpFrom _ _ = Some ?midx, H2: rsEdgeUpFrom _ _ = Some ?midx |- _] =>
-      assert (midx <> midx) by solve_midx_neq; auto
-    | [H1: rqEdgeUpFrom _ _ = Some ?midx, H2: edgeDownTo _ _ = Some ?midx |- _] =>
-      assert (midx <> midx) by solve_midx_neq; auto
-    | [H1: rsEdgeUpFrom _ _ = Some ?midx, H2: edgeDownTo _ _ = Some ?midx |- _] =>
-      assert (midx <> midx) by solve_midx_neq; auto
-    end.
-  
   Ltac disc_rule_custom ::=
     try disc_footprints_ok;
-    try exfalso_midx.
+    try solve_midx_false.
   
   Lemma step_inside_tree_ins_disj_outs:
     forall st1,
@@ -48,10 +38,7 @@ Section InsideTree.
     intros.
     destruct Hrrs as [? [? ?]].
     pose proof (footprints_ok H4 H).
-    red; intros [up umsg].
-    destruct (in_dec (id_dec msg_dec) (up, umsg) ups) as [Hin1|]; auto.
-    destruct (in_dec (id_dec msg_dec) (up, umsg) rins) as [Hin2|]; auto.
-    exfalso.
+    apply (DisjList_false_spec (id_dec msg_dec)); intros [up umsg] Hin1 Hin2.
     rewrite Forall_forall in H2.
     specialize (H2 _ Hin1); simpl in H2.
     
@@ -157,48 +144,232 @@ Section RqRsRed.
   Hypothesis (Hrrs: RqRsSys dtr sys).
 
   Lemma rqrs_lbl_ins_disj:
-    forall st1,
-      Reachable (steps step_m) sys st1 ->
-      forall oidx1 ridx1 rins1 routs1 oidx2 ridx2 rins2 routs2 st2,
+    forall st11 st21,
+      Reachable (steps step_m) sys st11 ->
+      Reachable (steps step_m) sys st21 ->
+      forall oidx1 ridx1 rins1 routs1 st12
+             oidx2 ridx2 rins2 routs2 st22,
         oidx1 <> oidx2 ->
-        steps step_m sys st1
-              [RlblInt oidx2 ridx2 rins2 routs2;
-                 RlblInt oidx1 ridx1 rins1 routs1] st2 ->
+        step_m sys st11 (RlblInt oidx1 ridx1 rins1 routs1) st12 ->
+        step_m sys st21 (RlblInt oidx2 ridx2 rins2 routs2) st22 ->
         DisjList (idsOf rins1) (idsOf rins2).
   Proof.
-  Admitted.
+    destruct Hrrs as [? [? ?]]; intros.
+    eapply messages_in_cases in H5; try eassumption.
+    eapply messages_in_cases in H6; try eassumption.
+
+    destruct H5 as [|[|[|]]]; destruct H6 as [|[|[|]]];
+      repeat disc_messages_in;
+      unfold idOf in *; simpl in *; solve_midx_disj;
+        try (intro Hx; rewrite Forall_forall in H6; specialize (H6 _ Hx);
+             destruct H6 as [rcidx ?]; dest;
+             solve_midx_false; fail).
+    - intro Hx; rewrite Hx in *; clear Hx.
+      repeat disc_rule_minds; auto.
+    - apply (DisjList_false_spec eq_nat_dec); intros midx Hin1 Hin2.
+      rewrite Forall_forall in H8; specialize (H8 _ Hin1).
+      destruct H8 as [cidx1 ?]; dest.
+      rewrite Forall_forall in H7; specialize (H7 _ Hin2).
+      destruct H7 as [cidx2 ?]; dest.
+      repeat disc_rule_minds; auto.
+    - intro Hx; rewrite Forall_forall in H7; specialize (H7 _ Hx).
+      destruct H7 as [rcidx ?]; dest.
+      solve_midx_false.
+    - intro Hx; rewrite Forall_forall in H7; specialize (H7 _ Hx).
+      destruct H7 as [rcidx ?]; dest.
+      solve_midx_false.
+  Qed.
 
   Lemma rqrs_lbl_outs_disj:
-    forall st1,
-      Reachable (steps step_m) sys st1 ->
-      forall oidx1 ridx1 rins1 routs1 oidx2 ridx2 rins2 routs2 st2,
+    forall st11 st21,
+      Reachable (steps step_m) sys st11 ->
+      Reachable (steps step_m) sys st21 ->
+      forall oidx1 ridx1 rins1 routs1 st12
+             oidx2 ridx2 rins2 routs2 st22,
         oidx1 <> oidx2 ->
-        steps step_m sys st1
-              [RlblInt oidx2 ridx2 rins2 routs2;
-                 RlblInt oidx1 ridx1 rins1 routs1] st2 ->
+        step_m sys st11 (RlblInt oidx1 ridx1 rins1 routs1) st12 ->
+        step_m sys st21 (RlblInt oidx2 ridx2 rins2 routs2) st22 ->
         DisjList (idsOf routs1) (idsOf routs2).
   Proof.
-  Admitted.
+    destruct Hrrs as [? [? ?]]; intros.
+    eapply messages_out_cases in H5; try eassumption.
+    eapply messages_out_cases in H6; try eassumption.
+
+    destruct H5 as [|[|[|]]]; destruct H6 as [|[|[|]]];
+      repeat disc_messages_out;
+      unfold idOf in *; simpl in *; solve_midx_disj;
+        try (intro Hx; rewrite Forall_forall in H7; specialize (H7 _ Hx);
+             destruct H7 as [rcidx ?]; dest;
+             (solve_midx_false || (repeat disc_rule_minds; auto));
+             fail).
+    - intro Hx; rewrite Forall_forall in H6; specialize (H6 _ Hx).
+      destruct H6 as [rcidx ?]; dest.
+      solve_midx_false.
+    - intro Hx; rewrite Forall_forall in H6; specialize (H6 _ Hx).
+      destruct H6 as [rcidx ?]; dest.
+      solve_midx_false.
+    - apply (DisjList_false_spec eq_nat_dec); intros midx Hin1 Hin2.
+      rewrite Forall_forall in H8; specialize (H8 _ Hin1).
+      destruct H8 as [cidx1 ?]; dest.
+      rewrite Forall_forall in H7; specialize (H7 _ Hin2).
+      destruct H7 as [cidx2 ?]; dest.
+      repeat disc_rule_minds; auto.
+    - intro Hx; rewrite Hx in *; clear Hx.
+      repeat disc_rule_minds; auto.
+  Qed.
+
+  Lemma rqrs_lbl_atomic_ins_disj:
+    forall inits1 ins1 hst1 outs1 eouts1,
+      Atomic msg_dec inits1 ins1 hst1 outs1 eouts1 ->
+      forall st11 st21,
+        Reachable (steps step_m) sys st11 ->
+        Reachable (steps step_m) sys st21 ->
+        forall oidx2 ridx2 rins2 routs2 st12 st22,
+          ~ In oidx2 (oindsOf hst1) ->
+          steps step_m sys st11 hst1 st12 ->
+          step_m sys st21 (RlblInt oidx2 ridx2 rins2 routs2) st22 ->
+          DisjList (idsOf ins1) (idsOf rins2).
+  Proof.
+    induction 1; simpl; intros; subst.
+    - inv_steps.
+      eapply rqrs_lbl_ins_disj; [| | |eassumption|eassumption]; eauto.
+    - inv_steps.
+      rewrite idsOf_app.
+      eapply DisjList_app_4; eauto.
+      eapply rqrs_lbl_ins_disj; [| | |eassumption|eassumption]; eauto.
+      eapply reachable_steps; [eapply H5|eassumption].
+  Qed.
 
   Lemma rqrs_atomic_ins_disj:
     forall inits1 ins1 hst1 outs1 eouts1 inits2 ins2 hst2 outs2 eouts2,
       Atomic msg_dec inits1 ins1 hst1 outs1 eouts1 ->
       Atomic msg_dec inits2 ins2 hst2 outs2 eouts2 ->
       DisjList (oindsOf hst1) (oindsOf hst2) ->
-      DisjList eouts1 inits2 ->
-      DisjList eouts1 ins2.
+      forall st11 st21,
+        Reachable (steps step_m) sys st11 ->
+        Reachable (steps step_m) sys st21 ->
+        forall st12 st22,
+          steps step_m sys st11 hst1 st12 ->
+          steps step_m sys st21 hst2 st22 ->
+          DisjList (idsOf ins1) (idsOf ins2).
   Proof.
-  Admitted.
+    induction 2; simpl; intros; subst.
+    - inv_steps.
+      eapply rqrs_lbl_atomic_ins_disj;
+        [| | | |eassumption|eassumption]; eauto.
+      specialize (H0 oidx); destruct H0; intuition.
+    - inv_steps.
+      apply DisjList_comm, DisjList_cons in H6; dest.
+      apply DisjList_comm in H4.
+      specialize (IHAtomic H4 _ _ H7 H8).
+      rewrite idsOf_app.
+      apply DisjList_comm, DisjList_app_4; apply DisjList_comm; eauto.
+      eapply rqrs_lbl_atomic_ins_disj;
+        [| | | |eapply H9|eapply H13]; eauto.
+  Qed.
+  
+  Lemma rqrs_lbl_atomic_outs_disj:
+    forall inits1 ins1 hst1 outs1 eouts1,
+      Atomic msg_dec inits1 ins1 hst1 outs1 eouts1 ->
+      forall st11 st21,
+        Reachable (steps step_m) sys st11 ->
+        Reachable (steps step_m) sys st21 ->
+        forall oidx2 ridx2 rins2 routs2 st12 st22,
+          ~ In oidx2 (oindsOf hst1) ->
+          steps step_m sys st11 hst1 st12 ->
+          step_m sys st21 (RlblInt oidx2 ridx2 rins2 routs2) st22 ->
+          DisjList (idsOf outs1) (idsOf routs2).
+  Proof.
+    induction 1; simpl; intros; subst.
+    - inv_steps.
+      eapply rqrs_lbl_outs_disj; [| | |eassumption|eassumption]; eauto.
+    - inv_steps.
+      rewrite idsOf_app.
+      eapply DisjList_app_4; eauto.
+      eapply rqrs_lbl_outs_disj; [| | |eassumption|eassumption]; eauto.
+      eapply reachable_steps; [eapply H5|eassumption].
+  Qed.
 
   Lemma rqrs_atomic_outs_disj:
     forall inits1 ins1 hst1 outs1 eouts1 inits2 ins2 hst2 outs2 eouts2,
       Atomic msg_dec inits1 ins1 hst1 outs1 eouts1 ->
       Atomic msg_dec inits2 ins2 hst2 outs2 eouts2 ->
       DisjList (oindsOf hst1) (oindsOf hst2) ->
-      DisjList eouts1 inits2 ->
-      DisjList outs1 inits2.
+      forall st11 st21,
+        Reachable (steps step_m) sys st11 ->
+        Reachable (steps step_m) sys st21 ->
+        forall st12 st22,
+          steps step_m sys st11 hst1 st12 ->
+          steps step_m sys st21 hst2 st22 ->
+          DisjList (idsOf outs1) (idsOf outs2).
   Proof.
-  Admitted.
+    induction 2; simpl; intros; subst.
+    - inv_steps.
+      eapply rqrs_lbl_atomic_outs_disj;
+        [| | | |eassumption|eassumption]; eauto.
+      specialize (H0 oidx); destruct H0; intuition.
+    - inv_steps.
+      apply DisjList_comm, DisjList_cons in H6; dest.
+      apply DisjList_comm in H4.
+      specialize (IHAtomic H4 _ _ H7 H8).
+      rewrite idsOf_app.
+      apply DisjList_comm, DisjList_app_4; apply DisjList_comm; eauto.
+      eapply rqrs_lbl_atomic_outs_disj;
+        [| | | |eapply H9|eapply H13]; eauto.
+  Qed.
+
+  Lemma rqrs_atomic_eouts_ins_disj:
+    forall inits1 ins1 hst1 outs1 eouts1 inits2 ins2 hst2 outs2 eouts2,
+      Atomic msg_dec inits1 ins1 hst1 outs1 eouts1 ->
+      Atomic msg_dec inits2 ins2 hst2 outs2 eouts2 ->
+      DisjList (oindsOf hst1) (oindsOf hst2) ->
+      DisjList eouts1 inits2 ->
+      forall st11 st21,
+        Reachable (steps step_m) sys st11 ->
+        Reachable (steps step_m) sys st21 ->
+        forall st12 st22,
+          steps step_m sys st11 hst1 st12 ->
+          steps step_m sys st21 hst2 st22 ->
+          DisjList eouts1 ins2.
+  Proof.
+    intros.
+    apply DisjList_app_1 with (l3:= eouts2).
+    eapply DisjList_comm, DisjList_SubList;
+      [eapply atomic_messages_ins_outs; eassumption|].
+    apply DisjList_app_4; [apply DisjList_comm; assumption|].
+    eapply DisjList_comm, DisjList_SubList;
+      [eapply atomic_eouts_in; eassumption|].
+    apply idsOf_DisjList.
+    eapply rqrs_atomic_outs_disj;
+      [eassumption|eassumption| | | |eassumption|eassumption]; eauto.
+  Qed.
+
+  Lemma rqrs_atomic_outs_inits_disj:
+    forall inits1 ins1 hst1 outs1 eouts1 inits2 ins2 hst2 outs2 eouts2,
+      Atomic msg_dec inits1 ins1 hst1 outs1 eouts1 ->
+      Atomic msg_dec inits2 ins2 hst2 outs2 eouts2 ->
+      DisjList (oindsOf hst1) (oindsOf hst2) ->
+      DisjList eouts1 inits2 ->
+      forall st11 st21,
+        Reachable (steps step_m) sys st11 ->
+        Reachable (steps step_m) sys st21 ->
+        forall st12 st22,
+          steps step_m sys st11 hst1 st12 ->
+          steps step_m sys st21 hst2 st22 ->
+          DisjList outs1 inits2.
+  Proof.
+    intros.
+    apply DisjList_comm, DisjList_app_2 with (l2:= inits1).
+    eapply DisjList_comm, DisjList_SubList;
+      [eapply atomic_messages_ins_outs in H; destruct H; eassumption|].
+    apply DisjList_app_4; [|assumption].
+    eapply DisjList_comm, DisjList_SubList;
+      [eapply atomic_inits_in; eassumption|].
+    apply DisjList_comm.
+    apply idsOf_DisjList.
+    eapply rqrs_atomic_ins_disj;
+      [eassumption|eassumption| | | |eassumption|eassumption]; eauto.
+  Qed.
 
   Lemma rqrs_lbl_reducible':
     forall inits1 ins1 hst1 outs1 eouts1 lbl2 oidx2 ridx2 rins2 routs2,
@@ -211,8 +382,14 @@ Section RqRsRed.
     unfold Reducible; induction 1; simpl; intros; subst.
     - apply internal_commutes; auto.
       + red; intuition.
-      + eapply rqrs_lbl_ins_disj; try eassumption; intuition.
-      + eapply rqrs_lbl_outs_disj; try eassumption; intuition.
+      + inv_steps.
+        eapply rqrs_lbl_ins_disj; [| | |eassumption|eassumption]; eauto.
+        eapply reachable_steps;
+          [eassumption|eapply steps_singleton; eassumption].
+      + inv_steps.
+        eapply rqrs_lbl_outs_disj; [| | |eassumption|eassumption]; eauto.
+        eapply reachable_steps;
+          [eassumption|eapply steps_singleton; eassumption].
     - eapply reducible_trans; try eassumption.
       + apply reducible_cons_2.
         * change (RlblInt oidx2 ridx2 rins2 routs2 :: RlblInt oidx ridx rins routs :: hst)
@@ -222,14 +399,16 @@ Section RqRsRed.
           destruct H8 as [sti [? ?]].
           apply internal_commutes; auto.
           { red; intuition. }
-          { eapply rqrs_lbl_ins_disj;
-              [eapply reachable_steps; eassumption| |eassumption].
-            intuition.
+          { inv_steps.
+            eapply rqrs_lbl_ins_disj; [| | |eassumption|eassumption]; eauto.
+            eapply reachable_steps; [|eapply steps_singleton; eassumption].
+            eapply reachable_steps; eassumption.
           }
           { eapply DisjList_app_3 in H7; dest; assumption. }
-          { eapply rqrs_lbl_outs_disj;
-              [eapply reachable_steps; eassumption| |eassumption].
-            intuition.
+          { inv_steps.
+            eapply rqrs_lbl_outs_disj; [| | |eassumption|eassumption]; eauto.
+            eapply reachable_steps; [|eapply steps_singleton; eassumption].
+            eapply reachable_steps; eassumption.
           }
       + apply reducible_cons.
         red; intros.
@@ -245,14 +424,20 @@ Section RqRsRed.
       DisjList eouts1 rins2 ->
       Reducible sys (lbl2 :: hst1) (hst1 ++ [lbl2]).
   Proof.
-    intros.
-    eapply rqrs_atomic_outs_disj with (outs1:= outs1) (hst2:= [lbl2]) in H2.
-    { eapply rqrs_lbl_reducible'; try eassumption. }
-    { eassumption. }
-    { subst; econstructor. }
-    { subst; simpl.
+    intros; red; intros.
+    inv_steps.
+    eapply rqrs_atomic_outs_inits_disj
+      with (outs1:= outs1) (hst2:= [RlblInt oidx2 ridx2 rins2 routs2]) in H2.
+    - eapply rqrs_lbl_reducible'; try eassumption; try reflexivity.
+      econstructor; eauto.
+    - eassumption.
+    - subst; econstructor.
+    - subst; simpl.
       apply (DisjList_singleton_2 eq_nat_dec); eassumption.
-    }
+    - eassumption.
+    - eapply reachable_steps; eassumption.
+    - eassumption.
+    - apply steps_singleton; eassumption.
   Qed.
 
   Lemma rqrs_reducible':
@@ -290,9 +475,19 @@ Section RqRsRed.
       DisjList eouts1 inits2 ->
       Reducible sys (hst2 ++ hst1) (hst1 ++ hst2).
   Proof.
-    intros.
-    eapply rqrs_atomic_ins_disj in H2; eauto; dest.
-    eapply rqrs_reducible'; eauto.
+    intros; red; intros.
+    eapply steps_split in H3; [|reflexivity].
+    destruct H3 as [sti [? ?]].
+    eapply rqrs_atomic_eouts_ins_disj in H2.
+    - eapply rqrs_reducible'; eauto.
+      eapply steps_append; eauto.
+    - eassumption.
+    - eassumption.
+    - assumption.
+    - eassumption.
+    - eapply reachable_steps; eassumption.
+    - eassumption.
+    - eassumption.
   Qed.
 
 End RqRsRed.
